theories/Sum.ec
@@ -6,25 +6,27 @@ require import Monoid.
 (* temporary workaround *)
 op intval : int -> int -> int set = interval.
 
-lemma intval_def : forall i i1 i2,
-  mem i (intval i1 i2)  <=> (i1<= i /\ i <= i2) by smt.
+lemma intval_def i i1 i2:
+  mem i (intval i1 i2)  <=> (i1<= i /\ i <= i2)
+by [].
 
-lemma intval_card_0 :
-  forall i1 (i2 : int), i1 <= i2 =>
-  card (intval i1 i2) = i2 - i1 + 1 by smt.
+lemma intval_card_0 i1 (i2 : int):
+  i1 <= i2 =>
+  card (intval i1 i2) = i2 - i1 + 1
+by [].
 
-lemma intval_card_1 :
-  forall i1 (i2:int), i2 < i1 => card (intval i1 i2) = 0 by smt.
+lemma intval_card_1 (i1 i2:int):
+  i2 < i1 => card (intval i1 i2) = 0
+by [].
 
-op int_sum : (int -> real) -> int set -> real = Mrplus.sum.
+op int_sum: (int -> real) -> int set -> real = Mrplus.sum.
 
 pred is_cnst (f : int -> 'a) = forall i1 i2, f i1 = f i2.
 
-lemma int_sum_const :
-  forall (f : int -> real) (s: int set), is_cnst f =>
-    int_sum f s = (card s)%r * f 0.
-intros f s cst.
-rewrite /int_sum (Mrplus.NatMul.sum_const (f 0)) //.
-intros x hh.
-by apply cst.
+lemma int_sum_const (f : int -> real) (s: int set):
+  is_cnst f => int_sum f s = (card s)%r * f 0.
+proof strict.
+by intros=> is_cnst;
+   rewrite /int_sum (Mrplus.NatMul.sum_const (f 0)) // => x hh;
+   apply is_cnst.
 qed.
